shift

src/common.lean
@@ -10,33 +10,240 @@
   
 namespace Parser
 
-  structure Ref (α : Type) where
-    internal : Nat
+  def Index (ls : List α) : Type := Fin (List.length ls)
+  private def Fin.max : Fin (Nat.succ k) := 0 - 1
+  def Index.new : Index (l :: ls) := Fin.max
+  private def Fin.ext : Fin k → Fin (k.succ)
+    | ⟨n, h⟩ => ⟨n, Nat.le_succ_of_le h⟩
+  
+  private theorem List.cons_get_eq (x : α) (xs : List α) (i : Index xs)
+    : (x :: xs).get i.succ = xs.get i := rfl
 
-  private inductive Syntax : Type → Type 1 where
-    | empty : Syntax α
+  structure Ref (tys : List Type) (α : Type) where
+    index : Index tys
+    same : tys.get index = α
+  namespace Ref
+    def tyPrepend {xs ys : List Type} (i : Index ys) : xs.length + i.val < (xs ++ ys).length :=
+      let goal : i.val < ys.length := i.isLt
+      let goal : xs.length + i.val < xs.length + ys.length :=
+        Nat.add_le_add_left goal xs.length
+      let goal : xs.length + i.val < (xs ++ ys).length :=
+        @Eq.subst _ (xs.length + i.val < .) _ _
+          (List.length_append xs ys).symm goal
+      goal
+    
+    def shift (newer : List Type) : Ref tys α → Ref (newer ++ tys) α
+      | { index := ⟨n, h⟩, same } =>
+        let i := ⟨n, h⟩
+        let index' := ⟨
+          newer.length + n,
+          Nat.add_lt_add_left h newer.length |> Eq.subst (List.length_append newer tys).symm
+        ⟩
+        {
+          index := index'
+          same := same |> @Eq.subst _ (λx => x = α) _ _
+            (getPrepend newer tys i : tys.get i = (newer ++ tys).get ⟨newer.length + i.val, _⟩)
+        }
+        where
+
+          getPrepend (xs : List Type)
+            : (ys : List Type) → (i : Index ys) -- → (h : xs.length + i.val < (xs ++ ys).length)
+            → ys.get i = (xs ++ ys).get ⟨xs.length + i.val, tyPrepend i⟩
+            | [y], ⟨0, h⟩ --, hxs
+              =>
+              let zero : Index [y] := ⟨0, h⟩
+              let h : xs.length + zero.val < (xs ++ [y]).length := tyPrepend zero
+              let rhs : Type := (xs ++ [y]).get ⟨xs.length, h⟩
+              let goal : rhs = rhs := rfl
+              let goal : y = rhs :=
+                let overrun : xs.length < xs.length → False := Nat.not_succ_le_self xs.length
+                @Eq.subst _ (. = rhs) ((xs ++ [y]).get ⟨xs.length, h⟩) _
+                  (List.get_last overrun) goal
+              let goal : ([] ++ [y]).get zero = rhs :=
+                let overrun (within : zero.val < [].length) : False := 
+                  let h : ¬zero.val < [].length := Nat.not_succ_le_self [].length
+                  absurd within h
+                @Eq.subst _ (. = rhs) y (([] ++ [y]).get zero)
+                  (List.get_last overrun).symm goal
+              let goal : [y].get zero = rhs :=
+                @Eq.subst ((ls : List Type) ×' Index ls) (λ⟨ls, i⟩ => ls.get i = rhs)
+                   ⟨[] ++ [y], ⟨0, _⟩⟩ ⟨[y], zero⟩
+                  (PSigma.eta (List.nil_append [y]) rfl) goal
+              goal
+            | (y :: ys), ⟨0, h⟩ --, h
+              =>
+              let zero : Index (y :: ys) := ⟨0, h⟩
+              let H (ls : List Type) : Prop := xs.length < ls.length
+              let h : H (xs ++ y :: ys) := tyPrepend zero
+              let i {ls : List Type} (h : H ls) : Index ls := ⟨xs.length, h⟩
+              let rhs : Type := (xs ++ y :: ys).get (i h)
+              let goal : (xs ++ y :: ys).get (i h) = rhs := rfl
+              let hOfAppends : H (xs ++ [y] ++ ys) :=
+                let goal : xs.length < xs.length.succ + ys.length :=
+                  Nat.le_add_right xs.length.succ ys.length
+                let goal : xs.length < xs.length + 1 + ys.length :=
+                  @Eq.subst _ (xs.length < . + ys.length) _ _
+                    (Nat.add_one xs.length).symm goal
+                let goal : xs.length < xs.length + [].length.succ + ys.length :=
+                  @Eq.subst _ (xs.length < xs.length + Nat.succ . + ys.length) _ _ List.length_nil.symm goal
+                let goal : xs.length < xs.length + [y].length + ys.length := goal
+                let goal : xs.length < (xs ++ [y]).length + ys.length :=
+                  @Eq.subst _ (xs.length < . + ys.length) _ _
+                    (List.length_append xs [y]).symm goal
+                let goal : xs.length < (xs ++ [y] ++ ys).length :=
+                  @Eq.subst _ (xs.length < .) _ _
+                    (List.length_append (xs ++ [y]) ys).symm goal
+                goal
+              let goal : (xs ++ [y] ++ ys).get (i hOfAppends) = rhs := 
+                @Eq.subst ((ls : List Type) ×' H ls) (λ⟨ls, h⟩ => ls.get (i h) = rhs)
+                   ⟨xs ++ y :: ys, h⟩ ⟨xs ++ [y] ++ ys, hOfAppends⟩
+                  (PSigma.eta (List.append_cons xs y ys) rfl) goal
+              let hOfSnoc : H (xs ++ [y]) := 
+                let goal : xs.length < xs.length.succ := Nat.succ_le_succ <| Nat.le_refl xs.length
+                let goal : xs.length < xs.length + [].length.succ :=
+                  @Eq.subst _ (xs.length < xs.length + Nat.succ .) _ _ List.length_nil.symm goal
+                let goal : xs.length < xs.length + [y].length := goal
+                let goal : xs.length < (xs ++ [y]).length :=
+                  @Eq.subst _ (xs.length < .) _ _
+                    (List.length_append xs [y]).symm goal
+                goal
+              let goal : (xs ++ [y]).get (i hOfSnoc) = rhs :=
+                @Eq.subst _ (. = rhs) _ _
+                  (List.get_append_left (xs ++ [y]) ys _) goal
+              let goal : y = rhs :=
+                let overrun : (i hOfSnoc).val < xs.length → False := Nat.not_succ_le_self xs.length
+                @Eq.subst _ (. = rhs) _ _
+                  (List.get_last overrun) goal
+              goal
+            | (y :: ys), ⟨Nat.succ k, h⟩ =>
+              let i : Index (y :: ys) := ⟨Nat.succ k, h⟩
+              let iPred : Index ys := ⟨k, Nat.le_of_succ_le_succ i.isLt⟩
+              let h : xs.length + i.val < (xs ++ y :: ys).length := tyPrepend i
+
+              let goal
+                : ys.get iPred = (xs ++ [y] ++ ys).get ⟨(xs ++ [y]).length + iPred.val, tyPrepend iPred⟩ :=
+                getPrepend (xs ++ [y]) ys iPred
+              let goal : ys.get iPred = (xs ++ y :: ys).get ⟨(xs ++ [y]).length + iPred.val, _⟩ :=
+                let h : (xs ++ [y]).length + iPred.val < (xs ++ y :: ys).length :=
+                  let goal : xs.length + iPred.val.succ < (xs ++ y :: ys).length := h
+                  let goal : xs.length + (iPred.val + 1) < (xs ++ y :: ys).length :=
+                    @Eq.subst _ (xs.length + . < (xs ++ y :: ys).length) _ _
+                      (Nat.succ_eq_add_one iPred.val) goal
+                  let goal : xs.length + (1 + iPred.val) < (xs ++ y :: ys).length :=
+                    @Eq.subst _ (xs.length + . < (xs ++ y :: ys).length) _ _
+                      (Nat.add_comm iPred.val 1) goal
+                  let goal : xs.length + 1 + iPred.val < (xs ++ y :: ys).length :=
+                    @Eq.subst _ (. < (xs ++ y :: ys).length) _ _
+                      (Nat.add_assoc xs.length 1 iPred.val).symm goal
+                  let goal : xs.length + [y].length + iPred.val < (xs ++ y :: ys).length := goal
+                  let goal : (xs ++ [y]).length + iPred.val < (xs ++ y :: ys).length :=
+                    @Eq.subst _ (. + iPred.val < (xs ++ y :: ys).length) _ _
+                      (List.length_append xs [y]).symm goal
+                  goal
+                @Eq.subst ((ls : List Type) ×' (xs ++ [y]).length + iPred.val < ls.length)
+                  (λ⟨ls, h⟩ => ys.get iPred = ls.get ⟨(xs ++ [y]).length + iPred.val, h⟩)
+                  ⟨xs ++ [y] ++ ys, tyPrepend iPred⟩ ⟨xs ++ y :: ys, h⟩
+                  (PSigma.eta (List.append_cons xs y ys).symm rfl) goal
+              let goal : ys.get iPred = (xs ++ y :: ys).get ⟨xs.length + [y].length + iPred.val, _⟩ :=
+                @Eq.subst ((n : Nat) ×' n + iPred.val < (xs ++ y :: ys).length)
+                  (λ⟨n, h⟩ => ys.get iPred = (xs ++ y :: ys).get ⟨n + iPred.val, h⟩)
+                  ⟨(xs ++ [y]).length, _⟩ ⟨xs.length + [y].length, _⟩
+                  (PSigma.eta (List.length_append xs [y]) rfl) goal
+              let goal : ys.get iPred = (xs ++ y :: ys).get ⟨xs.length + 1 + iPred.val, _⟩ := goal
+              let goal : ys.get iPred = (xs ++ y :: ys).get ⟨xs.length + (1 + iPred.val), _⟩ := 
+                @Eq.subst ((n : Nat) ×' n < (xs ++ y :: ys).length)
+                  (λ⟨n, h⟩ => ys.get iPred = (xs ++ y :: ys).get ⟨n, h⟩) _ _
+                  (PSigma.eta (Nat.add_assoc xs.length 1 iPred.val) rfl) goal
+              let goal : ys.get iPred = (xs ++ y :: ys).get ⟨xs.length + (iPred.val + 1), _⟩ :=
+                @Eq.subst ((n : Nat) ×' xs.length + n < (xs ++ y :: ys).length)
+                  (λ⟨n, h⟩ => ys.get iPred = (xs ++ y :: ys).get ⟨xs.length + n, h⟩) _ _
+                  (PSigma.eta (Nat.add_comm 1 iPred.val) rfl) goal
+              let goal : ys.get iPred = (xs ++ y :: ys).get ⟨xs.length + iPred.val.succ, _⟩ :=
+                @Eq.subst ((n : Nat) ×' xs.length + n < (xs ++ y :: ys).length)
+                  (λ⟨n, h⟩ => ys.get iPred = (xs ++ y :: ys).get ⟨xs.length + n, h⟩) _ _
+                  (PSigma.eta (Nat.add_one iPred.val) rfl) goal
+              let goal : ys.get iPred = (xs ++ y :: ys).get ⟨xs.length + i.val, h⟩ := goal
+              let goal : (y :: ys).get i = (xs ++ y :: ys).get ⟨xs.length + i.val, h⟩ := goal
+              goal
+
+  #check Eq.subst
+  #check False.rec
+
+    def ex : Ref [Char, Nat] Char := Ref.mk (Fin.ofNat 0 : Fin 2) rfl
+  end Ref
+
+  private inductive Syntax : List (Type) → Type → Type 1 where
+    | empty : Syntax (α :: tys) α
     -- -- | eps {α : Type} [inst : BEq α] [inst : Hashable α] : HashSet α → Parser' α
-    | eps : List α → Syntax α
-    | term (p : Char → Prop) [{a : Char} → Decidable (p a)] : Syntax Char
-    | or : Ref α → Ref α → Syntax α
-    | andThen : Ref α → Ref β → Syntax (α × β)
-    | map : (α → β) → Ref α → Syntax β
-    | null? : Ref α → Syntax α
+    | eps : List α → Syntax (α :: tys) α
+    | term (predicate : Char → Prop) [{a : Char} → Decidable (predicate a)]
+      : Syntax (Char :: tys) Char
+    | or (p : Ref pTys α) (q : Ref qTys α)
+      (pIsTail : tys.drop (tys.length - pTys.length) = pTys)
+      (qIsTail : tys.drop (tys.length - qTys.length) = qTys)
+      : Syntax (α :: tys) α
+    | andThen (p : Ref pTys α) (q : Ref qtys β)
+      (pIsTail : tys.drop (tys.length - pTys.length) = pTys)
+      (qIsTail : tys.drop (tys.length - qTys.length) = qTys)
+      : Syntax ((α × β) :: tys) (α × β)
+    | map : (α → β) → (p : Ref tys α) → Syntax (β :: tys) β
+    | isNull : (p : Ref tys α) → Syntax (α :: tys) α
+
+  -- instance [Repr α] [Repr β] [Repr (Syntax tys β)] : Repr (Syntax (ty :: tys) α) where
+  --   reprPrec
+  --     | Syntax.empty, _ => "empty"
+  --     | @Syntax.eps β tys parsed, prec => Repr.addAppParen ("eps " ++ reprArg parsed) prec
+  --     | Syntax.term predicate, prec => Repr.addAppParen "term {predicate}" prec
 
   inductive Memo : List Type → Type 1 where
     | empty : Memo []
-    | push : Memo tys → Syntax α → Memo (α :: tys) 
+    | push : Memo tys → Syntax (α :: tys) α → Memo (α :: tys)
   namespace Memo
 
-    def get : Memo tys → (i : Fin (List.length tys)) → Syntax (List.get tys i)
-      | push _ syn, ⟨0, _⟩ => syn
-      | push memo _, ⟨Nat.succ k, h⟩ => get memo ⟨k, Nat.le_of_succ_le_succ h⟩
+    def get : Memo tys → (ref : Ref tys α) → Syntax (tys.drop ref.index.val) α
+      | @push tysTail α _ s, Ref.mk ⟨0, _⟩ same => let tys := α :: tysTail
+        cast (congrArg (λα => Syntax tys α) same) s
+      | @push _ _ memo _, Ref.mk ⟨Nat.succ k, h⟩ same =>
+        get memo <| Ref.mk ⟨k, Nat.le_of_succ_le_succ h⟩ same
+
+  -- instance : Repr (Memo []) where
+  --   reprPrec
+  --     | Memo.empty, _ => "empty"
+
+  -- instance : Repr (Memo (ty :: tys)) where
+  --   reprPrec
+  --     | Memo.push memo syn, prec => Repr.addAppParen ("push " ++ reprArg memo ++ reprArg syn) prec
 
   end Memo
 
-  -- def Parser (α : Type) := StateM Memo <| Syntax α 
+  def Parser (tys : List Type) (α : Type) := Memo tys → (Ref (α :: tys) α × Memo (α :: tys))
 
-  -- def char (c : Char) : Parser Char := term (c = .)
+  def parser (syn : Syntax (α :: tys) α) : Parser tys α := λmemo =>
+    let h : 0 < (α :: tys).length :=
+      let goal : 0 < [α].length + tys.length := Nat.le_add_right 1 tys.length
+      let goal : 0 < ([α] ++ tys).length := Eq.subst (List.length_append [α] tys).symm goal
+      let goal : 0 < (α :: tys).length := goal
+      goal
+    (Ref.mk ⟨0, h⟩ rfl, memo.push syn)
+  def empty : Parser tys α := parser Syntax.empty
+  def eps : List α → Parser tys α := parser ∘ Syntax.eps
+  def term (predicate : Char → Prop) [inst : {a : Char} → Decidable (predicate a)]
+    : Parser tys Char := parser (Syntax.term predicate)
+  def or (p : Ref pTys α) (q : Ref qTys α)
+    (pIsTail : tys.drop (tys.length - pTys.length) = pTys)
+    (qIsTail : tys.drop (tys.length - qTys.length) = qTys)
+    : Parser tys α := parser (Syntax.or p q pIsTail qIsTail)
+  def map (f : α → β) (p : Ref tys α) : Parser tys β :=
+    parser (Syntax.map f p)
+
+  def char (c : Char) : Parser tys Char := term (c = .)
+
+  def ex : Parser [Char,Char] Char :=
+    let (p, memo) := char 'a' Memo.empty
+    let (q, memo) := char 'a' memo
+    or p q rfl rfl
+
+  #print ex
 
   -- -- private def printTest {α : Type} [Repr α] : (String ⊕ α) → IO Unit
   -- --   | (Sum.inr ok) => IO.println $ repr ok
@@ -188,4 +395,3 @@ namespace Parser
 --     spaces *> parser.many1 (parser.fix termF <* semicolon)
 
 end Parser
-export Parser (Parser)
